src/asn1/ASN1.Base.fst
@@ -38,7 +38,7 @@ let asn1_primitive_type
 /////      bounded mathematical integers for ASN1 value lengths
 ///// Defines the valid length/size of a ASN1 DER values
 ///////////////////////////////////////////////////////////////////////////
-let asn1_length_t = n: nat{0 <= n /\ n <= 4294967295}
+let asn1_length_t = n: nat{within_bounds (Unsigned W32) n}
 
 inline_for_extraction noextract
 let asn1_length_min: n: asn1_length_t {forall (n':asn1_length_t). n <= n'} = 0
