src/asn1/ASN1.Low.fst
@@ -1,6 +1,8 @@
 module ASN1.Low
 
+include ASN1.Base
 include ASN1.Low.Base
+include ASN1.Low.Bytes32
 include ASN1.Low.Tag
 include ASN1.Low.Length
 include ASN1.Low.Value
