src/asn1/ASN1.Spec.Bytes32.fst
@@ -1,0 +1,69 @@
+module ASN1.Spec.Bytes32
+
+open LowParse.Spec.Base
+open LowParse.Spec.Bytes
+open ASN1.Base
+
+open FStar.Integers
+module B32 = FStar.Bytes
+
+let parse_flbytes32_gen
+  (len: asn1_int32 )
+  (s: bytes { Seq.length s == v len } )
+: GTot (B32.lbytes32 len)
+= lt_pow2_32 (v len);
+  B32.hide s
+
+let parse_flbytes32
+  (len: asn1_int32 )
+: Tot (parser (total_constant_size_parser_kind (v len)) (B32.lbytes32 len))
+= make_total_constant_size_parser (v len) (B32.lbytes32 len) (parse_flbytes32_gen len)
+
+let serialize_flbytes32'
+  (len: asn1_int32)
+: Tot (bare_serializer (B32.lbytes32 len))
+= fun (x: B32.lbytes32 len) -> (
+    lt_pow2_32 (v len);
+    B32.reveal x
+  )
+
+#push-options "--query_stats --z3rlimit 16"
+let serialize_flbytes32_correct
+  (len: asn1_int32)
+: Lemma
+  (serializer_correct (parse_flbytes (v len)) (serialize_flbytes32' len))
+= let prf
+    (input: B32.lbytes32 len)
+  : Lemma
+    (
+      let ser = serialize_flbytes32' len input in
+      Seq.length ser == v len /\
+      parse (parse_flbytes32 len) ser == Some (input, (v len))
+    )
+  = ()
+  in
+  Classical.forall_intro prf
+
+let serialize_flbytes32
+  (len: asn1_int32)
+: Tot (serializer (parse_flbytes32 len))
+= serialize_flbytes32_correct len;
+  serialize_flbytes32' len
+
+let lemma_serialize_flbytes32_unfold
+  (len: asn1_int32)
+  (s32: B32.lbytes32 len)
+: Lemma (
+  serialize_flbytes32 len `serialize` s32 ==
+  B32.reveal s32
+)
+= ()
+
+let lemma_serialize_flbytes32_size
+  (len: asn1_int32)
+  (s32: B32.lbytes32 len)
+: Lemma (
+  Seq.length (serialize_flbytes32 len `serialize` s32) ==
+  v len
+)
+= ()
