src/asn1/ASN1.Spec.fst
@@ -2,6 +2,7 @@ module ASN1.Spec
 
 include ASN1.Base
 include ASN1.Spec.Base
+include ASN1.Spec.Bytes32
 include ASN1.Spec.Tag
 include ASN1.Spec.Length
 include ASN1.Spec.Value
