src/asn1/RIoT.X509.AliasKeyCRT.fst
@@ -1,0 +1,182 @@
+module RIoT.X509.AliasKeyCRT
+
+open ASN1.Spec
+open ASN1.Low
+open X509
+include RIoT.X509.Base
+include RIoT.X509.FWID
+include RIoT.X509.CompositeDeviceID
+include RIoT.X509.Extension
+open FStar.Integers
+
+module B32 = FStar.Bytes
+
+open LowParse.Spec.SeqBytes.Base
+open LowParse.Spec.Bytes
+
+#push-options "--query_stats --z3rlimit 32 --fuel 4 --ifuel 4"
+type aliasKeyCRT_t (tbs_len: asn1_int32) = {
+  aliasKeyCRT_tbs: B32.lbytes32 tbs_len;
+  aliasKeyCRT_sig_alg: algorithmIdentifier_t_inbound ED25519;
+  aliasKeyCRT_sig: x509_signature_t_inbound ED25519
+}
+#pop-options
+
+let aliasKeyCRT_t' (tbs_len: asn1_int32) = (
+  (B32.lbytes32 tbs_len `tuple2`
+   algorithmIdentifier_t_inbound ED25519) `tuple2`
+   x509_signature_t_inbound ED25519
+)
+
+let synth_aliasKeyCRT_t
+  (tbs_len: asn1_int32)
+  (x': aliasKeyCRT_t' tbs_len)
+: GTot (aliasKeyCRT_t tbs_len)
+= { aliasKeyCRT_tbs     = fst (fst x');
+    aliasKeyCRT_sig_alg = snd (fst x');
+    aliasKeyCRT_sig     = snd x' }
+
+let synth_aliasKeyCRT_t'
+  (tbs_len: asn1_int32)
+  (x: aliasKeyCRT_t tbs_len)
+: Tot (x': aliasKeyCRT_t' tbs_len { x == synth_aliasKeyCRT_t tbs_len x' })
+= (x.aliasKeyCRT_tbs,
+   x.aliasKeyCRT_sig_alg),
+   x.aliasKeyCRT_sig
+
+let parse_aliasKeyCRT
+  (tbs_len: asn1_int32)
+: parser _ (aliasKeyCRT_t tbs_len)
+= parse_flbytes32 tbs_len
+  `nondep_then`
+  parse_algorithmIdentifier_sequence_TLV ED25519
+  `nondep_then`
+  parse_x509_signature_sequence_TLV ED25519
+  `parse_synth`
+  synth_aliasKeyCRT_t tbs_len
+
+let serialize_aliasKeyCRT
+  (tbs_len: asn1_int32)
+: serializer (parse_aliasKeyCRT tbs_len)
+= serialize_synth
+  (* p1 *) (parse_flbytes32 tbs_len
+            `nondep_then`
+            parse_algorithmIdentifier_sequence_TLV ED25519
+            `nondep_then`
+            parse_x509_signature_sequence_TLV ED25519)
+  (* f2 *) (synth_aliasKeyCRT_t tbs_len)
+  (* s1 *) (serialize_flbytes32 tbs_len
+            `serialize_nondep_then`
+            serialize_algorithmIdentifier_sequence_TLV ED25519
+            `serialize_nondep_then`
+            serialize_x509_signature_sequence_TLV ED25519)
+  (* g1 *) (synth_aliasKeyCRT_t' tbs_len)
+  (* prf*) ()
+
+let lemma_serialize_aliasKeyCRT_unfold
+  (tbs_len: asn1_int32)
+  (x: aliasKeyCRT_t tbs_len)
+: Lemma (
+  serialize_aliasKeyCRT tbs_len `serialize` x ==
+ (serialize_flbytes32 tbs_len `serialize` x.aliasKeyCRT_tbs)
+  `Seq.append`
+ (serialize_algorithmIdentifier_sequence_TLV ED25519 `serialize` x.aliasKeyCRT_sig_alg)
+  `Seq.append`
+ (serialize_x509_signature_sequence_TLV ED25519 `serialize` x.aliasKeyCRT_sig)
+)
+= serialize_nondep_then_eq
+  (* s1 *) (serialize_flbytes32 tbs_len)
+  (* s2 *) (serialize_algorithmIdentifier_sequence_TLV ED25519)
+  (* in *) (fst (synth_aliasKeyCRT_t' tbs_len x));
+  serialize_nondep_then_eq
+  (* s1 *) (serialize_flbytes32 tbs_len
+            `serialize_nondep_then`
+            serialize_algorithmIdentifier_sequence_TLV ED25519)
+  (* s2 *) (serialize_x509_signature_sequence_TLV ED25519)
+  (* in *) (synth_aliasKeyCRT_t' tbs_len x);
+  serialize_synth_eq
+  (* p1 *) (parse_flbytes32 tbs_len
+            `nondep_then`
+            parse_algorithmIdentifier_sequence_TLV ED25519
+            `nondep_then`
+            parse_x509_signature_sequence_TLV ED25519)
+  (* f2 *) (synth_aliasKeyCRT_t tbs_len)
+  (* s1 *) (serialize_flbytes32 tbs_len
+            `serialize_nondep_then`
+            serialize_algorithmIdentifier_sequence_TLV ED25519
+            `serialize_nondep_then`
+            serialize_x509_signature_sequence_TLV ED25519)
+  (* g1 *) (synth_aliasKeyCRT_t' tbs_len)
+  (* prf*) ()
+  (* in *) x
+
+#restart-solver
+#push-options "--query_stats --z3rlimit 32" //--fuel 8 --ifuel 4"
+let lemma_serialize_aliasKeyCRT_size
+  (tbs_len: asn1_int32)
+  (x: aliasKeyCRT_t tbs_len)
+: Lemma (
+  length_of_opaque_serialization (serialize_aliasKeyCRT tbs_len) x ==
+  length_of_opaque_serialization (serialize_flbytes32 tbs_len) x.aliasKeyCRT_tbs +
+  length_of_opaque_serialization (serialize_algorithmIdentifier_sequence_TLV ED25519) x.aliasKeyCRT_sig_alg +
+  length_of_opaque_serialization (serialize_x509_signature_sequence_TLV ED25519) x.aliasKeyCRT_sig
+)
+= lemma_serialize_aliasKeyCRT_unfold tbs_len x
+#pop-options
+
+let aliasKeyCRT_t_inbound
+  (tbs_len: asn1_int32)
+= inbound_sequence_value_of (serialize_aliasKeyCRT tbs_len)
+
+let parse_aliasKeyCRT_sequence_TLV
+  (tbs_len: asn1_int32)
+: parser (parse_asn1_envelop_tag_with_TLV_kind SEQUENCE) (aliasKeyCRT_t_inbound tbs_len)
+= aliasKeyCRT_t_inbound tbs_len
+  `coerce_parser`
+  parse_asn1_sequence_TLV (serialize_aliasKeyCRT tbs_len)
+
+let serialize_aliasKeyCRT_sequence_TLV
+  (tbs_len: asn1_int32)
+: serializer (parse_aliasKeyCRT_sequence_TLV tbs_len)
+= coerce_parser_serializer
+    (parse_aliasKeyCRT_sequence_TLV tbs_len)
+    (serialize_asn1_sequence_TLV (serialize_aliasKeyCRT tbs_len))
+    ()
+
+let serialize_aliasKeyCRT_sequence_TLV_unfold
+  (tbs_len: asn1_int32)
+  (x: aliasKeyCRT_t_inbound tbs_len)
+: Lemma ( prop_serialize_asn1_sequence_TLV_unfold (serialize_aliasKeyCRT tbs_len) x )
+= lemma_serialize_asn1_sequence_TLV_unfold (serialize_aliasKeyCRT tbs_len) x
+
+let serialize_aliasKeyCRT_sequence_TLV_size
+  (tbs_len: asn1_int32)
+  (x: aliasKeyCRT_t_inbound tbs_len)
+: Lemma ( prop_serialize_asn1_sequence_TLV_size (serialize_aliasKeyCRT tbs_len) x )
+= lemma_serialize_asn1_sequence_TLV_size (serialize_aliasKeyCRT tbs_len) x
+
+(* low *)
+
+let serialize32_aliasKeyCRT_backwards
+  (tbs_len: asn1_int32)
+: serializer32_backwards (serialize_aliasKeyCRT tbs_len)
+= serialize32_synth_backwards
+  (* s1 *) (serialize32_flbytes32_backwards tbs_len
+            `serialize32_nondep_then_backwards`
+            serialize32_algorithmIdentifier_sequence_TLV_backwards ED25519
+            `serialize32_nondep_then_backwards`
+            serialize32_x509_signature_sequence_TLV_backwards ED25519)
+  (* f2 *) (synth_aliasKeyCRT_t  tbs_len)
+  (* g1 *) (synth_aliasKeyCRT_t' tbs_len)
+  (* g1'*) (synth_aliasKeyCRT_t' tbs_len)
+  (* prf*) ()
+
+let serialize32_aliasKeyCRT_sequence_TLV_backwards
+  (tbs_len: asn1_int32)
+: serializer32_backwards (serialize_aliasKeyCRT_sequence_TLV tbs_len)
+= coerce_serializer32_backwards
+    (serialize_aliasKeyCRT_sequence_TLV tbs_len)
+    (serialize32_asn1_sequence_TLV_backwards
+       (serialize32_aliasKeyCRT_backwards tbs_len))
+    ()
+
