src/asn1/RIoT.X509.AliasKeyTBS.fst
@@ -1,0 +1,250 @@
+module RIoT.X509.AliasKeyTBS
+
+open ASN1.Spec
+open ASN1.Low
+open X509
+include RIoT.X509.Base
+include RIoT.X509.FWID
+include RIoT.X509.CompositeDeviceID
+include RIoT.X509.Extension
+open FStar.Integers
+
+module B32 = FStar.Bytes
+
+open LowParse.Spec.SeqBytes.Base
+open LowParse.Spec.Bytes
+
+type aliasKeyTBS_t (header_len: asn1_int32) = {
+  aliasKeyTBS_header: B32.lbytes32 header_len;
+  aliasKeyTBS_aliasKey_pub: subjectPublicKeyInfo_t_inbound alg_AliasKey;
+  aliasKeyTBS_riot_extension: riot_extension_t_inbound;
+}
+
+let aliasKeyTBS_t' (header_len: asn1_int32) = (
+  (B32.lbytes32 header_len `tuple2`
+   subjectPublicKeyInfo_t_inbound alg_AliasKey) `tuple2`
+   riot_extension_t_inbound
+)
+
+let synth_aliasKeyTBS_t
+  (header_len: asn1_int32)
+  (x': aliasKeyTBS_t' header_len)
+: GTot (aliasKeyTBS_t header_len)
+= { aliasKeyTBS_header         = fst (fst x');
+    aliasKeyTBS_aliasKey_pub   = snd (fst x');
+    aliasKeyTBS_riot_extension = snd x' }
+
+let synth_aliasKeyTBS_t'
+  (header_len: asn1_int32)
+  (x: aliasKeyTBS_t header_len)
+: Tot (x': aliasKeyTBS_t' header_len { x == synth_aliasKeyTBS_t header_len x' })
+= (x.aliasKeyTBS_header,
+   x.aliasKeyTBS_aliasKey_pub),
+   x.aliasKeyTBS_riot_extension
+
+let parse_aliasKeyTBS
+  (header_len: asn1_int32)
+: parser _ (aliasKeyTBS_t header_len)
+= parse_flbytes32 header_len
+  `nondep_then`
+  parse_subjectPublicKeyInfo_sequence_TLV alg_AliasKey
+  `nondep_then`
+  parse_riot_extension_sequence_TLV
+  `parse_synth`
+  synth_aliasKeyTBS_t header_len
+
+let serialize_aliasKeyTBS
+  (header_len: asn1_int32)
+: serializer (parse_aliasKeyTBS header_len)
+= serialize_synth
+  (* p1 *) (parse_flbytes32 header_len
+            `nondep_then`
+            parse_subjectPublicKeyInfo_sequence_TLV alg_AliasKey
+            `nondep_then`
+            parse_riot_extension_sequence_TLV)
+  (* f2 *) (synth_aliasKeyTBS_t header_len)
+  (* s1 *) (serialize_flbytes32 header_len
+            `serialize_nondep_then`
+            serialize_subjectPublicKeyInfo_sequence_TLV alg_AliasKey
+            `serialize_nondep_then`
+            serialize_riot_extension_sequence_TLV)
+  (* g1 *) (synth_aliasKeyTBS_t' header_len)
+  (* prf*) ()
+
+let lemma_serialize_aliasKeyTBS_unfold
+  (header_len: asn1_int32)
+  (x: aliasKeyTBS_t header_len)
+: Lemma (
+  serialize_aliasKeyTBS header_len `serialize` x ==
+ (serialize_flbytes32 header_len `serialize` x.aliasKeyTBS_header)
+  `Seq.append`
+ (serialize_subjectPublicKeyInfo_sequence_TLV alg_AliasKey `serialize` x.aliasKeyTBS_aliasKey_pub)
+  `Seq.append`
+ (serialize_riot_extension_sequence_TLV `serialize` x.aliasKeyTBS_riot_extension)
+)
+= serialize_nondep_then_eq
+  (* s1 *) (serialize_flbytes32 header_len)
+  (* s2 *) (serialize_subjectPublicKeyInfo_sequence_TLV alg_AliasKey)
+  (* in *) (fst (synth_aliasKeyTBS_t' header_len x));
+  serialize_nondep_then_eq
+  (* s1 *) (serialize_flbytes32 header_len
+            `serialize_nondep_then`
+            serialize_subjectPublicKeyInfo_sequence_TLV alg_AliasKey)
+  (* s2 *) (serialize_riot_extension_sequence_TLV)
+  (* in *) (synth_aliasKeyTBS_t' header_len x);
+  serialize_synth_eq
+  (* p1 *) (parse_flbytes32 header_len
+            `nondep_then`
+            parse_subjectPublicKeyInfo_sequence_TLV alg_AliasKey
+            `nondep_then`
+            parse_riot_extension_sequence_TLV)
+  (* f2 *) (synth_aliasKeyTBS_t header_len)
+  (* s1 *) (serialize_flbytes32 header_len
+            `serialize_nondep_then`
+            serialize_subjectPublicKeyInfo_sequence_TLV alg_AliasKey
+            `serialize_nondep_then`
+            serialize_riot_extension_sequence_TLV)
+  (* g1 *) (synth_aliasKeyTBS_t' header_len)
+  (* prf*) ()
+  (* in *) x
+
+#restart-solver
+#push-options "--query_stats --z3rlimit 128 --fuel 8 --ifuel 4"
+let lemma_serialize_aliasKeyTBS_size
+  (header_len: asn1_int32)
+  (x: aliasKeyTBS_t header_len)
+: Lemma (
+  (* unfold *)
+  length_of_opaque_serialization (serialize_aliasKeyTBS header_len) x ==
+  length_of_opaque_serialization (serialize_flbytes32 header_len) x.aliasKeyTBS_header +
+  length_of_opaque_serialization (serialize_subjectPublicKeyInfo_sequence_TLV alg_AliasKey) x.aliasKeyTBS_aliasKey_pub +
+  length_of_opaque_serialization (serialize_riot_extension_sequence_TLV) x.aliasKeyTBS_riot_extension /\
+  (* exact size *)
+  length_of_opaque_serialization (serialize_aliasKeyTBS header_len) x
+  == v header_len + length_of_asn1_primitive_TLV x.aliasKeyTBS_riot_extension.x509_extValue.riot_version + 155 /\
+  (* upper bound *)
+  length_of_opaque_serialization (serialize_aliasKeyTBS header_len) x
+  <= v header_len + 161
+)
+= lemma_serialize_aliasKeyTBS_unfold header_len x;
+    lemma_serialize_subjectPublicKeyInfo_sequence_TLV_size_exact alg_AliasKey x.aliasKeyTBS_aliasKey_pub;
+    lemma_serialize_riot_extension_sequence_TLV_size_exact x.aliasKeyTBS_riot_extension
+#pop-options
+
+// unfold
+let aliasKeyTBS_t_inbound
+  (header_len: asn1_int32)
+= inbound_sequence_value_of (serialize_aliasKeyTBS header_len)
+
+let parse_aliasKeyTBS_sequence_TLV
+  (header_len: asn1_int32)
+: parser (parse_asn1_envelop_tag_with_TLV_kind SEQUENCE) (aliasKeyTBS_t_inbound header_len)
+=
+  aliasKeyTBS_t_inbound header_len
+  `coerce_parser`
+  parse_asn1_sequence_TLV (serialize_aliasKeyTBS header_len)
+
+let serialize_aliasKeyTBS_sequence_TLV
+  (header_len: asn1_int32)
+: serializer (parse_aliasKeyTBS_sequence_TLV header_len)
+= coerce_parser_serializer
+    (parse_aliasKeyTBS_sequence_TLV header_len)
+    (serialize_asn1_sequence_TLV (serialize_aliasKeyTBS header_len))
+    ()
+
+let lemma_serialize_aliasKeyTBS_sequence_TLV_unfold
+  (header_len: asn1_int32)
+  (x: aliasKeyTBS_t_inbound header_len)
+: Lemma ( prop_serialize_asn1_sequence_TLV_unfold (serialize_aliasKeyTBS header_len) x )
+= lemma_serialize_asn1_sequence_TLV_unfold (serialize_aliasKeyTBS header_len) x
+
+let lemma_serialize_aliasKeyTBS_sequence_TLV_size
+  (header_len: asn1_int32)
+  (x: aliasKeyTBS_t_inbound header_len)
+: Lemma ( prop_serialize_asn1_sequence_TLV_size (serialize_aliasKeyTBS header_len) x )
+= lemma_serialize_asn1_sequence_TLV_size (serialize_aliasKeyTBS header_len) x
+
+
+#restart-solver
+#push-options "--query_stats --z3rlimit 256 --fuel 8 --ifuel 4"
+let lemma_serialize_aliasKeyTBS_sequence_TLV_size_exact
+  (header_len: asn1_int32)
+  (x: aliasKeyTBS_t_inbound header_len)
+: Lemma (
+  let length = v header_len + length_of_asn1_primitive_TLV x.aliasKeyTBS_riot_extension.x509_extValue.riot_version + 155 in
+  length == length_of_opaque_serialization (serialize_aliasKeyTBS header_len) x /\
+  (* exact size *)
+  length_of_opaque_serialization (serialize_aliasKeyTBS_sequence_TLV header_len) x
+  == v header_len + length_of_asn1_primitive_TLV x.aliasKeyTBS_riot_extension.x509_extValue.riot_version + 156 +
+     length_of_asn1_length (u length) /\
+  (* upper bound *)
+  length_of_opaque_serialization (serialize_aliasKeyTBS_sequence_TLV header_len) x
+  <= v header_len + 167
+)
+= lemma_serialize_aliasKeyTBS_sequence_TLV_size header_len x;
+    lemma_serialize_aliasKeyTBS_size header_len x
+#pop-options
+
+(* low *)
+
+let serialize32_aliasKeyTBS_backwards
+  (header_len: asn1_int32)
+: serializer32_backwards (serialize_aliasKeyTBS header_len)
+= serialize32_synth_backwards
+  (* s1 *) (serialize32_flbytes32_backwards header_len
+            `serialize32_nondep_then_backwards`
+            serialize32_subjectPublicKeyInfo_sequence_TLV_backwards alg_AliasKey
+            `serialize32_nondep_then_backwards`
+            serialize32_riot_extension_sequence_TLV_backwards)
+  (* f2 *) (synth_aliasKeyTBS_t  header_len)
+  (* g1 *) (synth_aliasKeyTBS_t' header_len)
+  (* g1'*) (synth_aliasKeyTBS_t' header_len)
+  (* prf*) ()
+
+let serialize32_aliasKeyTBS_sequence_TLV_backwards
+  (header_len: asn1_int32)
+: serializer32_backwards (serialize_aliasKeyTBS_sequence_TLV header_len)
+= coerce_serializer32_backwards
+  (* s2 *) (serialize_aliasKeyTBS_sequence_TLV header_len)
+  (* s32*) (serialize32_asn1_sequence_TLV_backwards
+             (serialize32_aliasKeyTBS_backwards header_len))
+  (* prf*) ()
+
+
+(* helpers *)
+
+#restart-solver
+#push-options "--query_stats --z3rlimit 32 --initial_fuel 2 --ifuel 4"
+let x509_get_AliasKeyTBS
+  (header_len: asn1_int32)
+  (aliasKeyTBS_header: B32.lbytes32 header_len)
+  (version: datatype_of_asn1_type INTEGER
+            { v header_len + length_of_asn1_primitive_TLV version + 155
+             <= asn1_value_length_max_of_type SEQUENCE })
+  (fwid: B32.lbytes32 32ul)
+  (deviceIDPub: B32.lbytes32 32ul)
+  (aliasKeyPub: B32.lbytes32 32ul)
+: Tot (aliasKeyTBS_t_inbound header_len)
+=
+  let riot_extension= x509_get_riot_extension
+                        version
+                        fwid
+                        deviceIDPub in
+  (* Prf *) lemma_serialize_riot_extension_sequence_TLV_size_exact riot_extension;
+
+  let aliasKeyPubInfo = x509_get_subjectPublicKeyInfo
+                           alg_AliasKey
+                           aliasKeyPub in
+  (* Prf *) lemma_serialize_subjectPublicKeyInfo_sequence_TLV_size_exact alg_AliasKey aliasKeyPubInfo;
+
+  let aliasKeyTBS: aliasKeyTBS_t header_len = {
+    aliasKeyTBS_header         = aliasKeyTBS_header;
+    aliasKeyTBS_aliasKey_pub   = aliasKeyPubInfo;
+    aliasKeyTBS_riot_extension = riot_extension
+  } in
+  (* Prf *) lemma_serialize_aliasKeyTBS_unfold header_len aliasKeyTBS;
+  (* Prf *) lemma_serialize_aliasKeyTBS_size   header_len aliasKeyTBS;
+  (* Prf *) (**) lemma_serialize_flbytes32_size header_len aliasKeyTBS.aliasKeyTBS_header;
+
+(*return*) aliasKeyTBS
+#pop-options
